Correctness.thy
@@ -44,7 +44,7 @@ proof -
   with ED EN TD have ES: "iter (\<leadsto>\<^sub>k) (S\<^sub>k False [FReturn\<^sub>k] (unname e\<^sub>t)) (S\<^sub>k True [] (unname v\<^sub>t))" 
     by simp
   from TD have TC: "SE\<^sub>c [FReturn\<^sub>c []] [] (unname e\<^sub>t) :\<^sub>c t" 
-    by (metis tcc_state_ev tc\<^sub>c_nil tcc_snil tcc_scons_ret latest_environment.simps(4))
+    by (metisx tcc_state_ev tc\<^sub>c_nil tcc_snil tcc_scons_ret latest_environment.simps(4))
   with ES VD EN obtain c where EC: "iter (\<leadsto>\<^sub>c) (SE\<^sub>c [FReturn\<^sub>c []] [] (unname e\<^sub>t)) (SC\<^sub>c [] c) \<and> 
     declosure c = unname v\<^sub>t" by fastforce
   from TC EC have "iter (\<leadsto>\<^sub>e) (encode_state (SE\<^sub>c [FReturn\<^sub>c []] [] (unname e\<^sub>t))) 
